StlcPropV2.v
@@ -1,0 +1,111 @@
+Require Import SfLib.
+Require Import Maps.
+Require Import Types.
+Require Import Stlc.
+Require Import Smallstep.
+
+Module STLCPROP.
+Import STLC.
+
+Lemma canonical_forms_bool :
+forall t,
+    empty |- t \in TBool ->
+    value t ->
+    (t = ttrue) \/ (t = tfalse).
+
+    intros.
+    destruct t; inversion H0; try tauto.
+    inversion H.
+Qed.
+
+
+Lemma canonical_forms_fun :
+forall t T1 T2,
+    empty |- t \in (TArrow T1 T2) ->
+    value t ->
+    exists x u, t = tabs x T1 u.
+
+    intros. 
+    destruct t; inversion H0; try tauto; try (inversion H; fail).
+    exists i; exists t0. inversion H; auto.
+
+Qed.
+
+
+Theorem progress :
+forall t T,
+    empty |- t \in T ->
+    value t \/ exists t', t ==> t'.
+
+    intro. elim t; intros.
+    inversion H. inversion H2.
+    inversion H1. 
+    destruct (H (TArrow G T) H5);
+    destruct (H0 G H7); subst t0; subst t1; subst T.
+    inversion H8; inversion H9; subst t2; subst t3; try (try (inversion H5); try (inversion H1); fail).
+    inversion H7; subst G.   
+    right.  exists ([x0 := ttrue] y0 ). auto.
+    right; exists ([x0 := tfalse] y0); auto.
+    right; exists( [x0 := tabs x1 T1 y1] y0); auto.
+    destruct H9. right; exists (tapp t2 x0); auto.
+    destruct H8. right; exists (tapp x0 t3); auto.
+    destruct H8. right; exists (tapp x0 t3); auto.
+    left; auto.
+    left; auto. left ;auto.
+    right. inversion H2; subst t0; subst t1; subst t2; subst T.
+    destruct (H TBool H7).
+    inversion H3; try (subst t3; inversion H7).
+    exists t4; auto. exists t5; auto.
+    destruct H3. exists (tif x0 t4 t5); auto.
+Qed.
+
+
+
+
+Theorem preservation :
+forall t t' T,
+    empty |- t \in T ->
+    t ==> t' ->
+    empty |- t' \in T.
+
+    intro.
+    elim t.
+    intros. inversion H0. intros. inversion H2. subst abs; subst arg.
+    inversion H1. subst t0; subst t1; subst T0. pose(H abs' (TArrow G T) H8 H6).
+    eauto.
+    subst t1; subst t0; subst t'.
+    inversion H5; subst abs. inversion H1; inversion H8.
+    inversion H1; inversion H8.
+    inversion H1. subst t1;subst t2; subst T1. 
+    pose (H0 _ _ H10 H7). eauto.
+Abort.
+
+Lemma app_preserv:
+forall t g x G T,
+    empty |- tabs x G t \in TArrow G T ->
+    empty |- g \in G ->
+    empty |- [x := g] t \in T.
+
+    intro. elim t.
+    intros. inversion H; subst; unfold subst in *; unfold update in *; unfold t_update in *.
+    destruct (eq_id_dec); subst. inversion H; subst. unfold update in *; unfold t_update in *.
+    inversion H4; subst. rewrite eq_id_dec_id in H5. inversion H5; subst; auto.
+    inversion H3; subst.  destruct eq_id_dec ; subst; try contradict. destruct (n eq_refl).
+    auto.
+
+    intros. change (empty |- tapp ([x0 := g] t0) ([x0 := g] t1) \in T).
+    inversion H1; subst. inversion H5; subst. pose (T_Abs _ _ _ _ _ H7).
+    pose (H _ _ _ _ h H2). 
+    pose (T_Abs _ _ _ _ _ H9).
+    pose (H0 _ _ _ _ h1 H2). eauto.
+
+    intros. remember T. generalize Heqt2.
+    elim T; intros; subst. inversion H0.
+    Abort.
+
+
+
+
+
+
+
